WIP SelArray

ulib/experimental/Steel.SelArray.fst
@@ -1,21 +1,259 @@
 module Steel.SelArray
 
-let array t = ref (Seq.seq t)
+let array t = Seq.seq (ref t)
+let length #t a = Seq.length a
 
-let is_array r = ptr r
-let array_sel r = ptr_sel r
+let vnil_rewrite
+  (t: Type)
+  (x: t_of vemp)
+: GTot (Seq.lseq t 0)
+= Seq.empty
 
-let alloc x n =
+let vnil
+  (t: Type)
+: Pure vprop
+  (requires True)
+  (ensures (fun v -> t_of v == Seq.lseq t 0))
+= vrewrite vemp (vnil_rewrite t)
+
+let vcons_rewrite
+  (#t: Type)
+  (n: nat)
+  (r: ref t)
+  (v: vprop)
+  (sq: squash (t_of v == Seq.lseq t n))
+  (xy: t_of (vptr r `star` v))
+: GTot (Seq.lseq t (n + 1))
+= Seq.cons (fst xy) (snd xy)
+
+let vcons_rewrite_recip
+  (#t: Type)
+  (n: nat)
+  (r: ref t)
+  (v: vprop)
+  (sq: squash (t_of v == Seq.lseq t n))
+  (l: Seq.lseq t (n + 1))
+: GTot (t_of (vptr r `star` v))
+= (Seq.head l, Seq.tail l)
+
+let vcons_rewrite_recip_correct
+  (#t: Type)
+  (n: nat)
+  (r: ref t)
+  (v: vprop)
+  (sq: squash (t_of v == Seq.lseq t n))
+: Lemma
+  (elim_vrewrite_precond (vptr r `star` v) (vcons_rewrite n r v sq) (vcons_rewrite_recip n r v sq))
+  [SMTPat (elim_vrewrite_precond (vptr r `star` v) (vcons_rewrite n r v sq) (vcons_rewrite_recip n r v sq))]
+=
+  let g (xy: t_of (vptr r `star` v)) 
+    : Lemma
+      (vcons_rewrite_recip n r v sq (vcons_rewrite n r v sq xy) == xy)
+      [SMTPat (vcons_rewrite_recip n r v sq (vcons_rewrite n r v sq xy))]
+  = Seq.head_cons (fst xy) (snd xy);
+    Seq.lemma_tl (fst xy) (snd xy)
+  in
+  ()
+
+let vcons
+  (#t: Type)
+  (n: nat)
+  (r: ref t)
+  (v: vprop)
+: Pure vprop
+  (requires (t_of v == Seq.lseq t n))
+  (ensures (fun v' -> t_of v' == Seq.lseq t (n + 1)))
+= vrewrite (vptr r `star` v) (vcons_rewrite n r v ())
+
+let rec varray1
+  (#t: Type0)
+  (a: array t)
+: Pure vprop
+  (requires True)
+  (ensures (fun v -> t_of v == Seq.lseq t (length a)))
+  (decreases (length a))
+= if length a = 0
+  then vnil t
+  else vcons (Seq.length a - 1) (Seq.index a 0) (varray1 (Seq.slice a 1 (length a)))
+
+let is_array #a r = hp_of (varray1 r)
+
+let array_sel #a r = fun h -> sel_of (varray1 r) h
+
+let intro_varray
+  (#t: Type)
+  (r: array t)
+: SteelSel unit
+    (varray1 r)
+    (fun _ -> varray r)
+    (fun _ -> True)
+    (fun h _ h' -> h' (varray r) == h (varray1 r))
+=
+  let m = get #(varray1 r) () in
+  let x : Ghost.erased (t_of (varray1 r)) = Ghost.hide (m (varray1 r <: vprop)) in
+  let x' : Ghost.erased (Seq.lseq t (length r)) = Ghost.hide (Ghost.reveal x) in
+  change_slprop
+    (varray1 r)
+    (varray r)
+    x
+    x'
+    (fun _ -> ())
+
+#restart-solver
+
+unfold
+let coerce (#t1: Type) (x: t1) (t2: Type) : Pure t2
+  (requires (t1 == t2))
+  (ensures (fun y -> y == x))
+= x
+
+let elim_varray
+  (#t: Type)
+  (r: array t)
+: SteelSel unit
+    (varray r)
+    (fun _ -> varray1 r)
+    (fun _ -> True)
+    (fun h _ h' -> h' (varray1 r) == h (varray r))
+=
+  let m = get #(varray r) () in
+  let x : Ghost.erased (t_of (varray r)) = Ghost.hide (m (varray r)) in
+  assert (t_of (varray1 r) == t_of (varray r));
+  let x' : Ghost.erased (t_of (varray1 r)) = Ghost.hide (coerce (Ghost.reveal x) (t_of (varray1 r))) in
+  change_slprop
+    (varray r)
+    (varray1 r)
+    x
+    x'
+    (fun _ -> ())
+
+let intro_nil
+  (t: Type)
+: SteelSel (array t)
+    vemp
+    (fun r -> varray1 r)
+    (fun _ -> True)
+    (fun _ r _ -> length r == 0)
+=
+  intro_vrewrite vemp (vnil_rewrite t);
+  let r : array t = Seq.empty in
+  change_slprop
+    (vrewrite vemp (vnil_rewrite t))
+    (varray1 r)
+    (Ghost.hide (Seq.empty #t <: t_of (vrewrite vemp (vnil_rewrite t))))
+    (Ghost.hide (Seq.empty #t <: t_of (varray1 r)))
+    (fun _ -> ());
+  r
+
+let intro_vcons
+  (#t: Type)
+  (r: ref t)
+  (a: array t)
+: SteelSel (array t)
+    (vptr r `star` varray1 a)
+    (fun a' -> varray1 a')
+    (fun _ -> True)
+    (fun h a' h' ->
+      (coerce (h' (varray1 a')) (Seq.lseq t (Seq.length a')) <: Seq.seq t) ==
+        Seq.cons (h (vptr r)) (coerce (h (varray1 a)) (Seq.lseq t (length a)))
+    )
+=
+  reveal_star (vptr r) (varray1 a); // FIXME: WHY WHY WHY?
+  intro_vrewrite (vptr r `star` varray1 a) (vcons_rewrite (Seq.length a) r (varray1 a) ());
+  let a' : array t = Seq.cons r a in
+  Seq.head_cons r a;
+  Seq.lemma_tl r a;
+  change_equal_slprop
+    (vrewrite (vptr r `star` varray1 a) (vcons_rewrite (Seq.length a) r (varray1 a) ()))
+    (varray1 a');
+  a'
+
+#set-options "--ide_id_info_off" 
+
+#push-options "--z3rlimit 64 --ifuel 4" // --query_stats"
+
+#restart-solver
+
+let elim_vcons
+  (#t: Type)
+  (a: array t)
+: SteelSel (ref t & array t)
+    (varray1 a)
+    (fun res -> vptr (fst res) `star` varray1 (snd res))
+    (fun _ -> length a > 0)
+    (fun h res h' ->
+      length a > 0 /\
+      begin let s = coerce (h (varray1 a)) (Seq.lseq t (length a)) in
+      h' (vptr (fst res)) == Seq.head s /\
+      True // Seq.tail s `Seq.equal` coerce (h' (varray1 (snd res))) (Seq.lseq t (length (snd res)))
+      end
+    )
+=
+  let m0 = get #(varray1 a) () in
+  Seq.cons_head_tail (coerce (m0 (varray1 a)) (Seq.lseq t (length a)));
+  let a0 : Seq.seq (ref t) = a in
+  Seq.cons_head_tail a0;
+  let r = Seq.head a0 in
+  let q = Seq.tail a0 in
+  Seq.head_cons r q;
+  Seq.lemma_tl r q;
+  change_equal_slprop
+    (varray1 a)
+    (vrewrite (vptr (r) `star` varray1 (q)) (vcons_rewrite (Seq.length (q)) (r) (varray1 (q)) ()));
+  let m1 = get #(vrewrite (vptr (r) `star` varray1 (q)) (vcons_rewrite (Seq.length (q)) (r) (varray1 (q)) ())) () in
+  assert (coerce (m0 (varray1 a)) (Seq.lseq t (length a)) == coerce (m1 (vrewrite (vptr (r) `star` varray1 (q)) (vcons_rewrite (Seq.length (q)) (r) (varray1 (q)) ()))) (Seq.lseq t (length a)));
+  elim_vrewrite (vptr (r) `star` varray1 (q)) (vcons_rewrite (Seq.length (q)) (r) (varray1 (q)) ()) (vcons_rewrite_recip (Seq.length (q)) (r) (varray1 (q)) ());
+  reveal_star (vptr (r)) (varray1 (q));
+  let m = get #(vptr (r) `star` varray1 (q)) () in
+  Seq.head_cons (m (vptr (r))) (coerce (m (varray1 (q))) (Seq.lseq t (length (q))));
+  Seq.lemma_tl (m (vptr (r))) (coerce (m (varray1 (q))) (Seq.lseq t (length (q))));
+//  assume (m (varray1 q) == snd (m (vptr r `star` varray1 q)));
+//  assert (Seq.tail (coerce (m0 (varray1 a)) (Seq.lseq t (length a))) == coerce (m (varray1 q)) (Seq.lseq t (length q)));
+  let res : (ref t & array t) = (r, q) in
+  change_equal_slprop
+    (vptr (r) `star` varray1 (q))
+    (vptr (fst res) `star` varray1 (snd res));
+  reveal_star (vptr (fst res)) (varray1 (snd res));
+  sladmit ();
+  res
+
+#pop-options
+
+(* FIXME: refine the model with nontrivial boundaries. To do that, I will need fractional permissions. *)
+
+let boundary = unit
+let lhs #_ _ = ()
+let rhs #_ _ = ()
+let freeable_boundaries _ _ = true
+
+let join #t al ar = sladmit ()
+
+let split #t a i = sladmit ()
+
+let alloc x n = sladmit ()
+(*
   let s = Seq.create (U32.v n) x in
   alloc s
+*)
 
-let index r i =
+let index r i = sladmit ()
+(*
   let s = read r in
   Seq.index s (U32.v i)
+*)
 
-let upd r i x =
+let upd r i x = sladmit ()
+(*
   let s = read r in
   let s' = Seq.upd s (U32.v i) x in
   write r s'
+*)
 
-let free r = free r
+let free #t r =
+  reveal_vemp ();
+  let res : Ghost.erased (t_of vemp) = Ghost.hide (coerce () (t_of vemp)) in
+  change_slprop_2
+    (varray r)
+    (vemp)
+    res
+    (fun m -> intro_emp m)
